implementation of bfn with fifos implemented by two lists ... à la Okasaki Extraction from file bfn_fifo_2l.v gives good results

fifo.v
@@ -9,9 +9,28 @@
 (*         CeCILL v2 FREE SOFTWARE LICENSE AGREEMENT          *)
 (**************************************************************)
 
-Require Import List.
+Require Import List Arith Omega.
+
+Require Import wf_utils llist.
 
 Set Implicit Arguments.
+
+Section fifo_props.
+
+  Variables  (X Q : Type) (fifo_list : Q -> list X) 
+                          (fifo_nil : Q)
+                          (fifo_enq : Q -> X -> Q)
+                          (fifo_deq : forall q, fifo_list q <> nil -> X * Q)
+                          (fifo_void : Q -> bool).
+
+  Definition fifo_nil_prop := fifo_list fifo_nil = nil.
+  Definition fifo_enq_prop := forall q x, fifo_list (fifo_enq q x) = fifo_list q ++ x :: nil.
+  Definition fifo_deq_prop := forall q Hq, let (x,q') := @fifo_deq q Hq in fifo_list q = x::fifo_list q'.
+  Definition fifo_void_prop := forall q, fifo_void q = true <-> fifo_list q = nil.
+
+  Definition fifo_props := fifo_nil_prop /\ fifo_enq_prop /\ fifo_deq_prop /\ fifo_void_prop.
+
+End fifo_props.
 
 Record fifo (X : Type) := {
   Q :> Type;
@@ -20,10 +39,10 @@ Record fifo (X : Type) := {
   fifo_enq : Q -> X -> Q;
   fifo_deq : forall q, fifo_list q <> nil -> X * Q;
   fifo_void : Q -> bool;
-  fifo_nil_spec : fifo_list fifo_nil = nil;
-  fifo_enq_spec : forall q x, fifo_list (fifo_enq q x) = fifo_list q ++ x :: nil;
-  fifo_deq_spec : forall q Hq, let (x,q') := @fifo_deq q Hq in fifo_list q = x::fifo_list q';
-  fifo_void_spec : forall q, fifo_void q = true <-> fifo_list q = nil
+  fifo_nil_spec : fifo_nil_prop fifo_list fifo_nil;
+  fifo_enq_spec : fifo_enq_prop fifo_list fifo_enq;
+  fifo_deq_spec : fifo_deq_prop fifo_list fifo_deq;
+  fifo_void_spec : fifo_void_prop fifo_list fifo_void;
 }.
 
 Arguments fifo_list { X f }.
@@ -53,7 +72,7 @@ Section fifo_trivial.
 
   Definition fifo_trivial : fifo X.
   Proof.
-    exists Q fifo_list fifo_nil fifo_enq fifo_deq fifo_void; auto.
+    exists Q fifo_list fifo_nil fifo_enq fifo_deq fifo_void; red; auto.
     intros [ | ] Hq; simpl; auto; destruct Hq; reflexivity.
     intros [ | ]; simpl; split; auto; discriminate.
   Defined.
@@ -91,46 +110,78 @@ Section fifo_two_lists.
 
   Variable X : Type.
 
-  Implicit Type q : (list X * list X).
+  Definition fifo_2l := (list X * list X)%type.
+  Notation Q := fifo_2l.
 
-  Let Q := (list X * list X)%type.
-  Let fifo_list q := let (l,r) := q in r++rev l.
-  Let fifo_nil : Q := (nil,nil).
-  Let fifo_enq q x := let (l,r) := q in (x::l,r).
-  Let fifo_deq q (Hq : fifo_list q <> nil) : X * Q.
+  Implicit Type q : Q.
+
+  Definition fifo_2l_list q := let (l,r) := q in l++rev r.
+  Definition fifo_2l_nil : Q := (nil,nil).
+  Definition fifo_2l_enq q x := let (l,r) := q in (l,x::r).
+
+  Let fifo_2l_deq_rec q (Hq : fifo_2l_list q <> nil) : { c : X * Q | let (x,q') := c in fifo_2l_list q = x::fifo_2l_list q' }.
   Proof.
-    revert Hq.
-    refine (match q with 
-      | (l,x::r)  => fun _ => (x,(l,r))
-      | (l,nil)   => match rev_linear l as rl return rev_linear l = rl -> _ with
-        | nil   => fun H E => _
-        | x::rl => fun _ _ => (x,(nil,rl))
-      end eq_refl
-    end).
-    rewrite rev_linear_spec in H.
-    destruct E; auto.
-  Defined.
+    revert Hq; induction on q as fifo_deq with measure (length (fst q)+2*length (snd q)); intros Hq.
+    refine (match q as q' return q = q' -> _ with 
+      | (nil,r)   => fun E  => let (res,Hres) := fifo_deq (rev_linear r,nil) _ _ in exist _ res _
+      | (x::l,r)  => fun _  => exist _ (x,(l,r)) _
+    end eq_refl).
+    + subst; simpl.
+      rewrite rev_linear_spec, rev_length.
+      simpl in Hq; destruct r; simpl; try omega; destruct Hq; trivial.
+    + subst; simpl in Hq |- *.
+      rewrite rev_linear_spec, <- app_nil_end; auto.
+    + subst; destruct res as (x,q').
+      rewrite <- Hres; simpl.
+      rewrite rev_linear_spec, <- app_nil_end; trivial.
+    + subst; trivial.
+  Qed.
+
+  Definition fifo_2l_deq q Hq := proj1_sig (fifo_2l_deq_rec q Hq).
   
-  Let fifo_void q: bool :=
+  Definition fifo_2l_void q: bool :=
     match q with (nil,nil) => true | _ => false end.
+
+  Definition fifo_2l_nil_spec : fifo_nil_prop fifo_2l_list fifo_2l_nil.
+  Proof. red; auto. Qed.
+
+  Definition fifo_2l_enq_spec : fifo_enq_prop fifo_2l_list fifo_2l_enq.
+  Proof. intros (l,r) x; simpl; rewrite app_ass; auto. Qed.
+
+  Definition fifo_2l_deq_spec : fifo_deq_prop fifo_2l_list fifo_2l_deq.
+  Proof. intros q Hq; apply (proj2_sig (fifo_2l_deq_rec q Hq)). Qed.
+
+  Definition fifo_2l_void_spec : fifo_void_prop fifo_2l_list fifo_2l_void.
+  Proof.
+    intros ([ | x l],[ | y r]); simpl; split; auto; try discriminate.
+    generalize (rev r); clear r; intros [ | ]; discriminate.
+  Qed.
+
+  Hint Resolve fifo_2l_nil_spec fifo_2l_enq_spec fifo_2l_deq_spec fifo_2l_void_spec.
+
+  Theorem fifo_2l_spec : fifo_props fifo_2l_list fifo_2l_nil fifo_2l_enq fifo_2l_deq fifo_2l_void.
+  Proof. red; auto. Qed.
 
   Definition fifo_two_lists : fifo X.
   Proof.
-    exists Q fifo_list fifo_nil fifo_enq fifo_deq fifo_void; auto.
-    + intros (l,r) x; simpl; rewrite app_ass; auto.
-    + intros (l,[ | x r]); simpl; auto.
-      rewrite rev_linear_spec.
-      generalize (rev l); clear l; intros [ | x rl ].
-      * intros []; reflexivity.
-      * intros _; apply app_nil_end.
-    + intros (l,r); simpl.
-      destruct l as [ | x l ].
-      * destruct r; simpl; split; auto; discriminate.
-      * simpl. destruct r; destruct (rev l); split; discriminate.
+    exists Q fifo_2l_list fifo_2l_nil fifo_2l_enq fifo_2l_deq fifo_2l_void; apply fifo_2l_spec; auto.
   Defined.
 
 End fifo_two_lists.
 
+Arguments fifo_2l_nil {X}.
+
+Recursive Extraction fifo_two_lists.
+
 Section fifo_two_lazy_lists.
 
+  (** From "Simple and Efficient Purely Functional Queues and Deques" by Chris Okasaki *)
+
+  Variable X : Type.
+
+ 
+  
+
+
 End fifo_two_lazy_lists.
+
