llist.v
@@ -1,0 +1,182 @@
+(**************************************************************)
+(*   Copyright Dominique Larchey-Wendling [*]                 *)
+(*             Ralph Matthes [+]                              *)
+(*                                                            *)
+(*                             [*] Affiliation LORIA -- CNRS  *)
+(*                             [*] Affiliation IRIT -- CNRS   *)
+(**************************************************************)
+(*      This file is distributed under the terms of the       *)
+(*         CeCILL v2 FREE SOFTWARE LICENSE AGREEMENT          *)
+(**************************************************************)
+
+Require Import List Arith Omega Wellfounded Extraction.
+
+Set Implicit Arguments.
+
+Section llist.
+
+  (* G54DTP Dependently Typed Programming.
+    Introduction to coinductive types.
+    Venanzio Capretta, March 2011.
+  *)
+
+  Variable X : Type.
+
+  CoInductive llist : Type :=
+    | lnil: llist
+    | lcons: X -> llist -> llist.
+
+  (* We must define an explicit unfold operation. *)
+
+  Definition lunfold (l : llist) : llist :=
+    match l with
+      | lnil => lnil
+      | lcons a l' => lcons a l'
+    end.
+ 
+  (* The next function unfolds a lazy list several times:
+     the natural number n says how many.
+  *)
+
+  Fixpoint lunfold_many (l:llist) n : llist :=
+    match n with
+      | O    => l
+      | S n => match l with
+          | lnil      => lnil
+          | lcons a l => lcons a (lunfold_many l n)
+          end
+    end.
+
+  (* We can prove that the unfolding is equal to the original list. *)
+
+  Lemma lunfold_many_eq: forall n (l:llist), l = lunfold_many l n.
+  Proof.
+    induction n as [ | n IHn ].
+    + trivial.
+    + intros [ | x l ].
+      * trivial.
+      * simpl; f_equal; auto.
+  Qed.
+
+  (* Every finite list can be transformed into a lazy list. *)
+
+  Fixpoint list_llist l : llist :=
+    match l with
+      | nil  => lnil
+      | a::l => lcons a (list_llist l)
+    end.
+    
+  Fact list_llist_inj l m : list_llist l = list_llist m -> l = m.
+  Proof.
+    revert m; induction l as [ | x l IHl ]; intros [ | y m ]; auto; try discriminate.
+    simpl; intros H; inversion H; f_equal; auto.
+  Qed.
+    
+  Inductive lfin : llist -> Prop :=
+    | lfin_lnil :  lfin lnil
+    | lfin_lcons : forall a l, lfin l -> lfin (lcons a l).
+    
+  Fact lfin_inv a l : lfin (lcons a l) -> lfin l.
+  Proof. inversion 1; assumption. Defined.
+
+  Section llist_list.
+
+    Let llist_list_rec : forall l, lfin l -> { m | l = list_llist m }.
+    Proof.
+      refine (fix loop l Hl { struct Hl } := 
+        match l as l' return lfin l' -> { m | l' = list_llist m } with
+          | lnil      => fun H => exist _ nil _
+          | lcons x l => fun H => let (r,Hr) := loop l _ in exist _ (x::r) _
+        end Hl); subst; trivial.
+      inversion H; trivial.
+    Qed.
+  
+    Definition llist_list l Hl := proj1_sig (@llist_list_rec l Hl).
+  
+    Fact llist_list_spec l Hl : l = list_llist (@llist_list l Hl).
+    Proof. apply (proj2_sig (@llist_list_rec l Hl)). Qed.
+
+  End llist_list.
+  
+  Arguments llist_list : clear implicits.
+  
+  Fact llist_list_fix_0 H : llist_list lnil H = nil.
+  Proof.
+    generalize (llist_list_spec H); simpl.
+    generalize (llist_list _ H).
+    intros [|]; try discriminate; auto.
+  Qed.
+  
+  Fact llist_list_fix_1 x l H : llist_list (lcons x l) H = x::llist_list l (lfin_inv H).
+  Proof.
+    generalize (llist_list_spec H); simpl.
+    generalize (llist_list _ H).
+    intros [|]; try discriminate.
+    simpl.
+    intros G; inversion G; f_equal; auto.
+    apply list_llist_inj; rewrite <- H2.
+    apply llist_list_spec.
+  Qed.
+
+  Definition lfin_length l Hl := length (llist_list l Hl).
+
+  Arguments lfin_length : clear implicits.
+  
+  Fact lfin_length_fix_0 H : lfin_length lnil H = 0.
+  Proof. unfold lfin_length; rewrite llist_list_fix_0; auto. Qed.
+  
+  Fact lfin_length_fix_1 x l H : lfin_length (lcons x l) H = S (lfin_length l (lfin_inv H)).
+  Proof. unfold lfin_length; rewrite llist_list_fix_1; auto. Qed.
+  
+End llist.
+
+Arguments lnil {X}.
+Arguments llist_list {X}.
+Arguments lfin_length {X}.
+
+Section Rotate.
+
+  (* Rotate with lazy lists (with a non-informative "finiteness" predicate 
+     It seems the algorithm manipulates f a as lazy lists and r as a list ... no sure
+     or three lazy lists ? *)
+
+  Variable (X : Type).
+  
+  Implicit Type (f r : llist X) (a : list X).
+  
+  Let prec  f Hf r Hr := lfin_length r Hr = 1 + lfin_length f Hf.
+  Let rspec f Hf r Hr a m := m = llist_list f Hf++rev (llist_list r Hr)++a.
+  
+  Fixpoint rotate f r a (Hf : lfin f) (Hr : lfin r) { struct Hf } : @prec f Hf r Hr -> sig (@rspec f Hf r Hr a). 
+  Proof.
+    revert Hr.
+    refine (match r as r' return forall (Hr : lfin r'), @prec f Hf _ Hr  -> sig (@rspec f Hf r' Hr a) with
+      | lnil       => _
+      | lcons y r' => _ 
+    end); intros Hr' H.
+    { exfalso.
+      red in H.
+      rewrite lfin_length_fix_0 in H; discriminate. }
+    revert Hf H.
+    refine (match f as f' return forall (Hf' : lfin f'), @prec f' Hf' _ Hr' -> sig (rspec Hf' Hr' a) with
+      | lnil       => _
+      | lcons x f' => _
+    end); intros Hf' H.
+    + exists (y::a).
+      red in H |- *; revert H.
+      rewrite llist_list_fix_0, llist_list_fix_1, lfin_length_fix_0, lfin_length_fix_1.
+      destruct r'.
+      * rewrite llist_list_fix_0; trivial.
+      * rewrite lfin_length_fix_1; discriminate.
+    + refine (let (ro,Hro) := rotate f' r' (y::a) (lfin_inv Hf') (lfin_inv Hr') _ in exist _ (x::ro) _).
+      * red in H |- *; revert H.
+        repeat rewrite lfin_length_fix_1; intros; omega.
+      * red in Hro |- *; revert Hro.
+        repeat rewrite llist_list_fix_1; intros; subst.
+        simpl; rewrite app_ass; auto.
+  Defined.
+
+End Rotate.
+
+Recursive Extraction llist_list list_llist rotate.
+
